@prefix dc: <http://purl.org/dc/elements/1.1/> .
@prefix flint: <http://ontology.tno.nl/normengineering/flint#> .
@prefix mermaid: <https://data.rijksfinancien.nl/mermaid/model/def/> .
@prefix owl: <http://www.w3.org/2002/07/owl#> .
@prefix rdf: <http://www.w3.org/1999/02/22-rdf-syntax-ns#> .
@prefix rdfs: <http://www.w3.org/2000/01/rdf-schema#> .
@prefix src: <http://ontology.tno.nl/normengineering/source#> .
@prefix xsd: <http://www.w3.org/2001/XMLSchema#> .

<http://ontology.tno.nl/normengineering/flint> a owl:Ontology ;
    dc:description "First draft for the FLINT ontology." ;
    owl:versionIRI <http://ontology.tno.nl/normengineering/flint/0.7.0> ;
    owl:versionInfo "0.7.0" .

flint:comment a owl:DatatypeProperty ;
    rdfs:label "comment" ;
    rdfs:comment "A note to explain modeling choices or issues with respect to a frame." ;
    rdfs:domain flint:Frame ;
    rdfs:range xsd:string ;
    rdfs:subPropertyOf rdfs:comment ;
    mermaid:label "http://ontology.tno.nl/normengineering/flint#Frame -- comment --> http://www.w3.org/2001/XMLSchema#string:::Datatype" ;
    mermaid:syntax "DATATYPEPROPERTY" .

flint:creates a owl:ObjectProperty ;
    rdfs:label "creates" ;
    rdfs:comment "Connects acts to those facts that it creates when it is performed." ;
    rdfs:domain flint:Act ;
    rdfs:range flint:AtomicFact ;
    rdfs:subPropertyOf owl:topObjectProperty ;
    owl:inverseOf flint:isCreatedBy ;
    mermaid:label "http://ontology.tno.nl/normengineering/flint#Act -- creates --> http://ontology.tno.nl/normengineering/flint#AtomicFact" ;
    mermaid:syntax "OBJECTPROPERTY" .

flint:hasAction a owl:ObjectProperty ;
    rdfs:label "Has action" ;
    rdfs:domain flint:Act ;
    rdfs:range flint:Action ;
    rdfs:subPropertyOf owl:topObjectProperty ;
    mermaid:label "http://ontology.tno.nl/normengineering/flint#Act -- hasAction --> http://ontology.tno.nl/normengineering/flint#Action" ;
    mermaid:syntax "OBJECTPROPERTY" .

flint:hasActor a owl:ObjectProperty ;
    rdfs:label "Has actor" ;
    rdfs:comment "The agent that can perform the act." ;
    rdfs:domain flint:Act ;
    rdfs:range flint:Agent ;
    rdfs:subPropertyOf owl:topObjectProperty ;
    mermaid:label "http://ontology.tno.nl/normengineering/flint#Act -- hasActor --> http://ontology.tno.nl/normengineering/flint#Agent" ;
    mermaid:syntax "OBJECTPROPERTY" .

flint:hasClaimant a owl:ObjectProperty ;
    rdfs:label "Has claimant" ;
    rdfs:comment "The agent holding the claim." ;
    rdfs:domain flint:Duty ;
    rdfs:range flint:Agent ;
    rdfs:subPropertyOf owl:topObjectProperty ;
    mermaid:label "http://ontology.tno.nl/normengineering/flint#Duty -- hasClaimant --> http://ontology.tno.nl/normengineering/flint#Agent" ;
    mermaid:syntax "OBJECTPROPERTY" .

flint:hasHolder a owl:ObjectProperty ;
    rdfs:label "Has holder" ;
    rdfs:comment "The agent holding the duty." ;
    rdfs:domain flint:Duty ;
    rdfs:range flint:Agent ;
    rdfs:subPropertyOf owl:topObjectProperty ;
    mermaid:label "http://ontology.tno.nl/normengineering/flint#Duty -- hasHolder --> http://ontology.tno.nl/normengineering/flint#Agent" ;
    mermaid:syntax "OBJECTPROPERTY" .

flint:hasObject a owl:ObjectProperty ;
    rdfs:label "Has object" ;
    rdfs:comment "The object acted upon" ;
    rdfs:domain flint:Act ;
    rdfs:range flint:Object ;
    rdfs:subPropertyOf owl:topObjectProperty ;
    mermaid:label "http://ontology.tno.nl/normengineering/flint#Act -- hasObject --> http://ontology.tno.nl/normengineering/flint#Object" ;
    mermaid:syntax "OBJECTPROPERTY" .

flint:hasPrecondition a owl:ObjectProperty ;
    rdfs:label "has precondition" ;
    rdfs:comment "Connects acts to (possibly complex) facts that must be true for the act to be valid." ;
    rdfs:domain flint:Act ;
    rdfs:range flint:Fact ;
    rdfs:subPropertyOf owl:topObjectProperty ;
    mermaid:label "http://ontology.tno.nl/normengineering/flint#Act -- hasPrecondition --> http://ontology.tno.nl/normengineering/flint#Fact" ;
    mermaid:syntax "OBJECTPROPERTY" .

flint:hasRecipient a owl:ObjectProperty ;
    rdfs:label "Has recipient" ;
    rdfs:comment "Recipient or interested party with respect to the act." ;
    rdfs:domain flint:Act ;
    rdfs:range flint:Agent ;
    rdfs:subPropertyOf owl:topObjectProperty ;
    mermaid:label "http://ontology.tno.nl/normengineering/flint#Act -- hasRecipient --> http://ontology.tno.nl/normengineering/flint#Agent" ;
    mermaid:syntax "OBJECTPROPERTY" .

flint:hasSource a owl:ObjectProperty ;
    rdfs:label "has source" ;
    rdfs:comment "Connects an act or fact to a structural element of a legal source" ;
    rdfs:domain flint:Frame ;
    rdfs:range src:Element ;
    rdfs:subPropertyOf owl:topObjectProperty ;
    mermaid:label "http://ontology.tno.nl/normengineering/flint#Frame -- hasSource --> http://ontology.tno.nl/normengineering/source#Element" ;
    mermaid:syntax "OBJECTPROPERTY" .

flint:hasTextFragment a owl:ObjectProperty ;
    rdfs:label "has text fragment" ;
    rdfs:comment "Connects an act or fact to a text fragment in a legal source." ;
    rdfs:domain flint:Frame ;
    rdfs:range src:TextFragment ;
    rdfs:subPropertyOf owl:topObjectProperty ;
    mermaid:label "http://ontology.tno.nl/normengineering/flint#Frame -- hasTextFragment --> http://ontology.tno.nl/normengineering/source#TextFragment" ;
    mermaid:syntax "OBJECTPROPERTY" .

flint:isTerminatedBy a owl:ObjectProperty ;
    rdfs:label "is terminated by" ;
    rdfs:comment "Connects facts to the acts that terminate it." ;
    rdfs:range flint:Act ;
    rdfs:subPropertyOf owl:topObjectProperty ;
    owl:inverseOf flint:terminates ;
    mermaid:syntax "OBJECTPROPERTY" .

flint:Action a owl:Class ;
    rdfs:label "Action" ;
    rdfs:comment "The type of action associated with an act (usually corresponds to the verb in the source text)." ;
    rdfs:subClassOf flint:Fact ;
    mermaid:label """http://ontology.tno.nl/normengineering/flint#Action((Action)) -- subClassOf --> http://ontology.tno.nl/normengineering/flint#Fact
""" ;
    mermaid:syntax "SUBCLASSOF" .

flint:Object a owl:Class ;
    rdfs:label "Object" ;
    rdfs:comment "The object of an act." ;
    rdfs:subClassOf flint:Fact ;
    mermaid:label """http://ontology.tno.nl/normengineering/flint#Object((Object)) -- subClassOf --> http://ontology.tno.nl/normengineering/flint#Fact
""" ;
    mermaid:syntax "SUBCLASSOF" .

flint:hasOperand a owl:ObjectProperty ;
    rdfs:label "Has operand" ;
    rdfs:comment "Connects a complex fact with its subfacts." ;
    rdfs:domain flint:ComplexFact ;
    rdfs:range flint:Fact ;
    rdfs:subPropertyOf owl:topObjectProperty ;
    mermaid:label "http://ontology.tno.nl/normengineering/flint#ComplexFact -- hasOperand --> http://ontology.tno.nl/normengineering/flint#Fact" ;
    mermaid:syntax "OBJECTPROPERTY" .

flint:isCreatedBy a owl:ObjectProperty ;
    rdfs:label "is created by" ;
    rdfs:comment "Connects facts to the acts that create it." ;
    rdfs:range flint:Act ;
    rdfs:subPropertyOf owl:topObjectProperty ;
    mermaid:syntax "OBJECTPROPERTY" .

flint:terminates a owl:ObjectProperty ;
    rdfs:label "terminates" ;
    rdfs:comment "Connects acts to those facts that it terminates when it is performed." ;
    rdfs:domain flint:Act ;
    rdfs:range flint:AtomicFact ;
    rdfs:subPropertyOf owl:topObjectProperty ;
    mermaid:label "http://ontology.tno.nl/normengineering/flint#Act -- terminates --> http://ontology.tno.nl/normengineering/flint#AtomicFact" ;
    mermaid:syntax "OBJECTPROPERTY" .

flint:AtomicFact a owl:Class ;
    rdfs:label "Atomic fact" ;
    rdfs:comment "Any fact that is not a complex fact. This can also be an agent or object." ;
    rdfs:subClassOf flint:Fact ;
    owl:disjointWith flint:ComplexFact ;
    mermaid:label """http://ontology.tno.nl/normengineering/flint#AtomicFact((AtomicFact)) -- subClassOf --> http://ontology.tno.nl/normengineering/flint#Fact
""" ;
    mermaid:syntax "SUBCLASSOF" .

flint:ConjunctiveFact a owl:Class ;
    rdfs:label "Conjunctive fact" ;
    rdfs:comment "A fact that is built up from other facts, connected by a conjunction (AND)." ;
    rdfs:subClassOf flint:ComplexFact ;
    owl:disjointWith flint:DisjunctiveFact,
        flint:NegatedFact ;
    mermaid:label """http://ontology.tno.nl/normengineering/flint#ConjunctiveFact((ConjunctiveFact)) -- subClassOf --> http://ontology.tno.nl/normengineering/flint#ComplexFact
""" ;
    mermaid:syntax "SUBCLASSOF" .

flint:DisjunctiveFact a owl:Class ;
    rdfs:label "Disjunctive fact" ;
    rdfs:comment "A fact that is built up from other facts, connected by a disjunction (OR)." ;
    rdfs:subClassOf flint:ComplexFact ;
    owl:disjointWith flint:ConjunctiveFact,
        flint:NegatedFact ;
    mermaid:label """http://ontology.tno.nl/normengineering/flint#DisjunctiveFact((DisjunctiveFact)) -- subClassOf --> http://ontology.tno.nl/normengineering/flint#ComplexFact
""" ;
    mermaid:syntax "SUBCLASSOF" .

flint:Duty a owl:Class ;
    rdfs:label "Duty" ;
    rdfs:comment "Describes a duty that should be performed by a duty holder for the benefit of a claimant." ;
    rdfs:subClassOf flint:Fact ;
    mermaid:label """http://ontology.tno.nl/normengineering/flint#Duty((Duty)) -- subClassOf --> http://ontology.tno.nl/normengineering/flint#Fact
""" ;
    mermaid:syntax "SUBCLASSOF" .

flint:NegatedFact a owl:Class ;
    rdfs:label "Negated fact" ;
    rdfs:comment "A fact that is the negation of another fact (NOT)." ;
    rdfs:subClassOf flint:ComplexFact ;
    owl:disjointWith flint:ConjunctiveFact,
        flint:DisjunctiveFact ;
    mermaid:label """http://ontology.tno.nl/normengineering/flint#NegatedFact((NegatedFact)) -- subClassOf --> http://ontology.tno.nl/normengineering/flint#ComplexFact
""" ;
    mermaid:syntax "SUBCLASSOF" .

flint:Agent a owl:Class ;
    rdfs:label "Agent" ;
    rdfs:comment "An agent is a duty holder, duty claimant, actor or act recipient." ;
    rdfs:subClassOf flint:Fact ;
    mermaid:label """http://ontology.tno.nl/normengineering/flint#Agent((Agent)) -- subClassOf --> http://ontology.tno.nl/normengineering/flint#Fact
""" ;
    mermaid:syntax "SUBCLASSOF" .

flint:ComplexFact a owl:Class ;
    rdfs:label "Complex fact" ;
    rdfs:comment "A fact that is built up from one or more other facts, connected by a boolean operator." ;
    rdfs:subClassOf flint:Fact ;
    owl:intersectionOf ( flint:Fact [ a owl:Restriction ;
                owl:onProperty flint:hasOperand ;
                owl:someValuesFrom flint:Fact ;
                mermaid:label """subgraph nb605b42198654d36b26661b801b1af5eb1[Restriction &exist; R C]
nb605b42198654d36b26661b801b1af5eb1thing((thing)) -- hasOperand some --> nb605b42198654d36b26661b801b1af5eb1http://ontology.tno.nl/normengineering/flint#Fact((Fact))

end
""" ;
                mermaid:syntax "SOME" ] ) ;
    mermaid:label """http://ontology.tno.nl/normengineering/flint#ComplexFact((ComplexFact)) -- equivalentTo --> http://ontology.tno.nl/normengineering/flint#ComplexFactc1e15344061d45b26ed41055886ed6a7c985b69e66078feacebb9aed0891d2b9
subgraph http://ontology.tno.nl/normengineering/flint#ComplexFactc1e15344061d45b26ed41055886ed6a7c985b69e66078feacebb9aed0891d2b9 [Intersection C &cap; D]
http://ontology.tno.nl/normengineering/flint#ComplexFacthttp://ontology.tno.nl/normengineering/flint#Fact((Fact)) -- and --- nb605b42198654d36b26661b801b1af5eb1
end
""",
        """http://ontology.tno.nl/normengineering/flint#ComplexFact((ComplexFact)) -- subClassOf --> http://ontology.tno.nl/normengineering/flint#Fact
""" ;
    mermaid:syntax "AND",
        "SUBCLASSOF" .

flint:Frame a owl:Class ;
    rdfs:label "Frame" ;
    rdfs:comment "An act or fact." ;
    mermaid:label "http://ontology.tno.nl/normengineering/flint#Frame((Frame))" ;
    mermaid:syntax "CLASS" .

flint:Act a owl:Class ;
    rdfs:label "Act" ;
    rdfs:comment "Describes an act that can be performed by an actor if its preconditions are met, and which results in creating and/or terminating facts." ;
    rdfs:subClassOf flint:Frame ;
    owl:disjointWith flint:Fact ;
    mermaid:label """http://ontology.tno.nl/normengineering/flint#Act((Act)) -- subClassOf --> http://ontology.tno.nl/normengineering/flint#Frame
""" ;
    mermaid:syntax "SUBCLASSOF" .

flint:Fact a owl:Class ;
    rdfs:label "Fact" ;
    rdfs:comment "Describes a fact that can serve as precondition, postcondition, agent or object." ;
    rdfs:subClassOf flint:Frame ;
    owl:disjointWith flint:Act ;
    mermaid:label """http://ontology.tno.nl/normengineering/flint#Fact((Fact)) -- subClassOf --> http://ontology.tno.nl/normengineering/flint#Frame
""" ;
    mermaid:syntax "SUBCLASSOF" .

